#@prefix : <> . Need to add a prefix for this namespace after setting up the namespace.
@prefix cco: <http://www.ontologyrepository.com/CommonCoreOntologies/> .
@prefix obo: <http://purl.obolibrary.org/obo/> .
@prefix owl: <http://www.w3.org/2002/07/owl#> .
@prefix rdf: <http://www.w3.org/1999/02/22-rdf-syntax-ns#> .
@prefix rdfs: <http://www.w3.org/2000/01/rdf-schema#> .
@prefix skos: <http://www.w3.org/2004/02/skos/core#> .
@prefix xml: <http://www.w3.org/XML/1998/namespace> .
@prefix xsd: <http://www.w3.org/2001/XMLSchema#> .
# @base <> . Once again, must create a namespace as the base of the ontology




########
#Classes
########

:0000001 
  a owl:Class ;
  rdfs:subClassOf obo:BFO_00000004 ;
  rdfs:label "MTG Object"@en ;
  skos:prefLabel "Object"@en ;
  skos:definition "An MTG object is an independent continuant which is either an ability on the stack, a card, a copy of a card, a token, a spell, a permanent, or an emblem."@en ;
  skos:note "This class is, of necessity, a defined class." ;
  skos:note "CR 109.1" ;
.

:0000002
  a owl:Class ;
  rdfs:subClassOf cco:Agent ;
  rdfs:label "MTG Player"@en ;
  skos:prefLabel "Player"@en ;
  skos:definition "An MTG player is an agent who is playing a game of Magic: the Gathering."@en ;
  skos:note "Players are often referred to in card text and can be targeted by certain effects. Thus, this term is not intended to refer to players in the colloquial sense of 'individual who sometimes plays such-and-such a game." ;
.

:0000003
  a owl:Class;
  rdfs:subClassOf obo:BFO_0000029 ;
  rdfs:label "MTG Zone"@en ;
  skos:prefLabel "Zone"@en ;
  skos:definition "A zone is a site where objects can be during a game."@en ;
  skos:note "The zone classes in MTG are library, hand, stack, battlefield, graveyard, exile, command, and ante." ;
  skos:note "this term should indicate a more general zone term for a mid-level games or card games ontology" ;
.

:0000004
  a owl:Class ;
  rdfs:subClassOf obo:BFO_0000015 ;
  rdfs:Label "MTG Game"@en ;
  skos:prefLabel "Game"@en ;
  skos:definition "A MTG game is a process that consists of players taking turns until one player wins the game"@en ;
  skos:note "this is a super loose definition, and this class should probably be subsumed under a more specific class, 'game', rather than BFO's process class. That, however, is beyond the scope of this project, and if you are unsure as to why, go read Wittgenstein or any philosophy of games." ;
.

:0000005
  a owl:Class ;
  rdfs:subClassOf obo:BFO_0000015 ;
  rdfs:Label "MTG Game Action" @en ;
  skos:prefLabel "Action"@en ;
  skos: altLabel "Game Action"@en ;
.

:0000006
  a owl:Class ;
  rdfs:subClassOf obo:BFO_0000015 ;
  rdfs:label "MTG Turn Process"@en ;
  skos:definition ""@en ;
  skos:note "" ;
.

:0000007
  a owl:Class ;
  rdfs:subClassOf :0000001 ;
  rdfs:label "Ability on the stack"@en ;
  skos:definition "An ability on the stack is an object which..."@en ;
.

:0000008
  a owl:Class ;
  owl:disjointWith :0000010 ;
  rdfs:subClassOf :0000001 ;
  rdfs:label "MTG Card"@en ;
  skos:definition "A card is an object which bears name, mana cost, illustration, color indicator, type line, expansion symbol, text box, power and toughness, loyalty, defense, hand modifier, life modifier, illustration credit, legal text, and collector number information."@en ;
  skos:altLabel "Magic Card"@en ;
  skos:prefLabel "Card"@en ;
  skos:note "CR 200.1" ;
.

:0000009
  a owl:Class ;
  rdfs:subClassOf :0000001 ; 
  rdfs:label "Copy" ;
  skos:definition "A Copy is an object whose characteristics are determined by some other object's characteristics, as chosen by a player in casting a spell, activating an ability, or resolving an effect."@en ;
.

:0000010
  a owl:Class ;
  owl:disjointWith :0000008 ;
  rdfs:subClassOf :0000001 ;
  rdfs:label "MTG Token" ;
  skos:definition "A token is a permanent that isn't a card."@en ;
  skos:prefLabel "Token"@en ;
  skos:note "CR 111.1" ;
.

:0000011
  a owl:Class ;
  rdfs:subClassOf :0000001 ;
  rdfs:label "MTG Spell"@en ;
  skos:definition "A spell is a card (or a copy of a card) that is on the stack."@en ;
  skos:prefLabel "Spell"@en ;
  skos:note "CR 112.1" ;
.

:0000012
  a owl:Class ;
  rdfs:subClassOf :0000001 ,
    [rdf:type owl:Restriction ;
              owl:onProperty obo:RO_0001025 ;
              owl:allValuesFrom :0000016
    ] ,
  rdfs:label "MTG Permanent"@en ;
  skos:definition "A permanent is a card or token that is on the battlefield."@en ;
  skos:prefLabel "Permanent"@en ;
  skos:note "CR 110.1" ;
.

:0000013
  a owl:Class ;
rdfs:subClassOf :0000001 ;
rdfs:label "MTG Emblem" ;
skos:definition "An Emblem is an object that has one or more abilities, but no other characteristics."@en ;
skos:prefLabel "Emblem"@em ;
skos:note "CR 114.1" ;
.

:0000014
  a owl:Class ;
  rdfs:subClassOf :0000003 ;
  rdfs:label "MTG Library Zone"@en ;
  skos:definition "A library is a zone in which a player's deck is placed in a face-down pile during a game."@en ;
  skos:prefLabel "Library"@en ;
  skos:note "CR 401" ;
.

:0000015
  a owl:Class ;
  rdfs:subClassOf :0000003 ;
  rdfs:label "MTG Hand Zone"@en ;
  skos:definition "A hand zone is a zone in which a player holds any cards they have drawn."@en ;
  skos:prefLabel "Hand"@en ;
  skos:note "CR 402" ;
.

:0000016
  a owl:Class ;
  rdfs:subClassOf :0000003 ;
  rdfs:label "MTG Battlefield Zone"@en ;
  skos:definition "The battlefield is the zone where permanents exist."@en ;
  skos:prefLabel "Battlefield"@en ;
  skos:note "CR 403" ;
.

:0000017
  a owl:Class ;
  rdfs:subClassOf :0000003 ;
  rdfs:label "MTG Graveyard Zone"@en ;
  skos:definition "A graveyard zone is a zone where objects owned by one player are placed on top of any objects already in that player's graveyard zone when they are countered, discarded, destroyed, milled, or sacrificed, or, in the case of instants and sorcery spells, after they resolve."@en ;
  skos:prefLabel "Graveyard"@en ;
  skos:note "CR 404" ;
.

:0000018
  a owl:Class ;
  rdfs:subClassOf :0000003 ;
  rdfs:label "MTG Exile Zone"@en ;
  skos:definition "The exile zone is a zone where objects can be placed."@en ;
  skos:prefLabel "Exile"@en ;
  skos:note "CR 406" ;
.

:0000019
  a owl:class ;
  rdfs:subClassOf :0000003 ;
  rdfs:label "MTG Stack Zone"@en ;
  skos:definition "The stack is a zone where cards and abilities are placed on top of each other in the order in which they are cast, activated, or triggered, and resolved in reverse order."@en ;
  skos:prefLabel "Stack"@en ;
  skos:note "CR 408" ;
.

:0000020
  a owl:Class ;
  rdfs:subClassOf :0000003 ;
  rdfs:label "MTG Command Zone"@en ;
  skos:definition "The command zone is a zone reserved for certain specialized objects that have an overarching effect on the game, yet are not permanents and cannot be destroyed."@en ;
  skos:prefLabel "Command Zone"@en ;
  skos:altLabel "Command" @en ;
  skos:note "CR 408" ;
  skos:note "The definition of this term may need to be tinkered with." ;
.

:0000021
  a owl:Class ;
  rdfs:subClassOf :0000003 ;
  rdfs:label "MTG Ante Zone"@en ;
  skos:definition "The ante zone is a zone that, after determining which player goes first but before drawing any cards, each player places one random card from their deck into, when playing for ante. The winner of the game becomes owner of any cards in the ante zone."@en ;
  skos:prefLabel "Ante Zone"@en ;
  skos:note "The ante zone does not get used much, is considered an optional rule, and probably only still exists in the rules because certain cards from early on in the game's history make reference to it" ;
  skos:note "CR 407" ;
.



##################
#Object Properties
##################

