#@prefix : <> . Need to add a prefix for this namespace after setting up the namespace.
@prefix cco: <http://www.ontologyrepository.com/CommonCoreOntologies/> .
@prefix obo: <http://purl.obolibrary.org/obo/> .
@prefix owl: <http://www.w3.org/2002/07/owl#> .
@prefix rdf: <http://www.w3.org/1999/02/22-rdf-syntax-ns#> .
@prefix rdfs: <http://www.w3.org/2000/01/rdf-schema#> .
@prefix skos: <http://www.w3.org/2004/02/skos/core#> .
@prefix xml: <http://www.w3.org/XML/1998/namespace> .
@prefix xsd: <http://www.w3.org/2001/XMLSchema#> .
# @base <> . Once again, must create a namespace as the base of the ontology




########
#Classes
########

:0000001 
  a owl:Class ;
  rdfs:subClassOf obo:BFO_00000002 ;
  rdfs:label "MTG Object"@en ;
  skos:prefLabel "Object"@en ;
  skos:definition "An MTG object is an independent continuant which is either an ability on the stack, a card, a copy of a card, a token, a spell, a permanent, or an emblem."@en ;
  skos:note "This class is, of necessity, a defined class." ;
  skos:note "CR 109.1" ;
.

:0000002
  a owl:Class ;
  rdfs:subClassOf cco:Agent ;
  rdfs:label "MTG Player"@en ;
  skos:prefLabel "Player"@en ;
  skos:definition "A MTG player is an agent realizing a player role in a game of Magic: the Gathering."@en ;
  skos:note "Players are often referred to in card text and can be targeted by certain effects. Thus, this term is not intended to refer to players in the colloquial sense of 'individual who sometimes plays such-and-such a game." ;
.

:0000003
  a owl:Class;
  rdfs:subClassOf obo:BFO_0000029 ;
  rdfs:label "MTG Zone"@en ;
  skos:prefLabel "Zone"@en ;
  skos:definition "A zone is a site where objects can be during a game."@en ;
  skos:note "The zone classes in MTG are library, hand, stack, battlefield, graveyard, exile, command, and ante." ;
  skos:note "this term should indicate a more general zone term for a mid-level games or card games ontology" ;
.

:0000004
  a owl:Class ;
  rdfs:subClassOf obo:BFO_0000015 ;
  rdfs:Label "MTG Game"@en ;
  skos:prefLabel "Game"@en ;
  skos:definition "A MTG game is a process that consists of players taking turns until a player(s) wins the game."@en ;
  skos:note "this is a super loose definition, and this class should probably be subsumed under a more specific class, 'game', rather than BFO's process class. That, however, is beyond the scope of this project, and if you are unsure as to why, go read Wittgenstein or any philosophy of games." ;
.

:0000005
  a owl:Class ;
  rdfs:subClassOf obo:BFO_0000015 ;
  rdfs:Label "MTG Game Action" @en ;
  skos:prefLabel "Action"@en ;
  skos: altLabel "Game Action"@en ;
  skos:definition "A game action is a process with at least a player and an object as participants, which has as its output a changed game state."@en ;
  skos:note "(Elucidation) Game actions should include things like casting spells, playing lands, activating abilities, resolving spells or abilities, drawing a card, tapping sources for mana, declaring attackers, and declaring blockers." ;
.

:0000006
  a owl:Class ;
  rdfs:subClassOf obo:BFO_0000015 ;
  rdfs:label "MTG Turn Process"@en ;
  skos:definition "A turn is a process that consists of the following phases, in this order: beginning phase, precombat main phase, combat phase, postcombat main phase, and end phase."@en ;
  skos:note "This should possibly point to a more general class of turns for any turn-based game." ;
.

:0000007
  a owl:Class ;
  rdfs:subClassOf :0000001 ;
  rdfs:label "Ability Object"@en ;
  skos:definition "An ability object is an object in the stack zone whose only object characteristic is a text box containing object ability information."@en ;
  skos:altLabel "Ability on the stack"@en ;
  skos:altLabel "Ability"@en ;
.

:0000008
  a owl:Class ;
  owl:disjointWith :0000010 ;
  rdfs:subClassOf :0000001 ;
  rdfs:label "MTG Card"@en ;
  skos:definition "A card is an object which bears name, mana cost, illustration, color indicator, type line, expansion symbol, text box, power and toughness, loyalty, defense, hand modifier, life modifier, illustration credit, legal text, and collector number information."@en ;
  skos:altLabel "Magic Card"@en ;
  skos:prefLabel "Card"@en ;
  skos:note "CR 200.1" ;
  skos:note "This is a problematic definition, enumerating the different kinds of information that can be borne by cards and making it sound as though all cards carry all of these. In particular, very few cards bear hand and life modifier information, because only specialized cards for a single format use those." ;
.

:0000009
  a owl:Class ;
  rdfs:subClassOf :0000001 ; 
  rdfs:label "Copy" ;
  skos:definition "A Copy is an object whose characteristics are determined by some other object's characteristics, as chosen by a player in casting a spell, activating an ability, or resolving an effect."@en ;
.

:0000010
  a owl:Class ;
  owl:disjointWith :0000008 ;
  rdfs:subClassOf :0000001 ;
  rdfs:label "MTG Token" ;
  skos:definition "A token is a permanent that isn't a card."@en ;
  skos:prefLabel "Token"@en ;
  skos:note "CR 111.1" ;
.

:0000011
  a owl:Class ;
  rdfs:subClassOf :0000001 ;
  rdfs:label "MTG Spell"@en ;
  skos:definition "A spell is a card (or a copy of a card) that is on the stack."@en ;
  skos:prefLabel "Spell"@en ;
  skos:note "CR 112.1" ;
.

:0000012
  a owl:Class ;
  rdfs:subClassOf :0000001 ,
    [rdf:type owl:Restriction ;
              owl:onProperty obo:RO_0001025 ;
              owl:allValuesFrom :0000016
    ] ;
  rdfs:label "MTG Permanent"@en ;
  skos:definition "A permanent is an object that is on the battlefield."@en ;
  skos:prefLabel "Permanent"@en ;
  skos:note "CR 110.1" ;
.

:0000013
  a owl:Class ;
rdfs:subClassOf :0000001 ,
    [rdf:type owl:Restriction ;
              owl:onProperty obo:RO_0001025 ;
              owl:allValuesFrom :0000020
    ] ,
    [rdf:type owl:Restriction ;
              owl:onProperty obo:BFO_0000101 ;
              owl:allValuesFrom :0000032
    ] ;
rdfs:label "MTG Emblem" ;
skos:definition "An Emblem is an object that has one or more abilities, but no other characteristics."@en ;
skos:prefLabel "Emblem"@em ;
skos:note "CR 114.1" ;
skos:note "During a game, emblems exist in the command zone (CR 114.2). This is why the first class restriction exists." ;
.

:0000014
  a owl:Class ;
  rdfs:subClassOf :0000003 ;
  rdfs:label "MTG Library Zone"@en ;
  skos:definition "A library is a zone in which a player's deck is placed in a face-down pile during a game."@en ;
  skos:prefLabel "Library"@en ;
  skos:note "CR 401" ;
.

:0000015
  a owl:Class ;
  rdfs:subClassOf :0000003 ;
  rdfs:label "MTG Hand Zone"@en ;
  skos:definition "A hand zone is a zone in which a player holds any cards they have drawn."@en ;
  skos:prefLabel "Hand"@en ;
  skos:note "CR 402" ;
.

:0000016
  a owl:Class ;
  rdfs:subClassOf :0000003 ;
  rdfs:label "MTG Battlefield Zone"@en ;
  skos:definition "The battlefield is the zone where permanents exist."@en ;
  skos:prefLabel "Battlefield"@en ;
  skos:note "CR 403" ;
.

:0000017
  a owl:Class ;
  rdfs:subClassOf :0000003 ;
  rdfs:label "MTG Graveyard Zone"@en ;
  skos:definition "A graveyard zone is a zone where objects owned by one player are placed on top of any objects already in that player's graveyard zone when they are countered, discarded, destroyed, milled, or sacrificed, or, in the case of instants and sorcery spells, after they resolve."@en ;
  skos:prefLabel "Graveyard"@en ;
  skos:note "CR 404" ;
.

:0000018
  a owl:Class ;
  rdfs:subClassOf :0000003 ;
  rdfs:label "MTG Exile Zone"@en ;
  skos:definition "The exile zone is a zone where objects can be placed."@en ;
  skos:prefLabel "Exile"@en ;
  skos:note "CR 406" ;
.

:0000019
  a owl:class ;
  rdfs:subClassOf :0000003 ;
  rdfs:label "MTG Stack Zone"@en ;
  skos:definition "The stack is a zone where cards and abilities are placed on top of each other in the order in which they are cast, activated, or triggered, and resolved in reverse order."@en ;
  skos:prefLabel "Stack"@en ;
  skos:note "CR 408" ;
.

:0000020
  a owl:Class ;
  rdfs:subClassOf :0000003 ;
  rdfs:label "MTG Command Zone"@en ;
  skos:definition "The command zone is a zone reserved for certain specialized objects that have an overarching effect on the game, yet are not permanents and cannot be destroyed."@en ;
  skos:prefLabel "Command Zone"@en ;
  skos:altLabel "Command" @en ;
  skos:note "CR 408" ;
  skos:note "The definition of this term may need to be tinkered with." ;
.

:0000021
  a owl:Class ;
  rdfs:subClassOf :0000003 ;
  rdfs:label "MTG Ante Zone"@en ;
  skos:definition "The ante zone is a zone that, after determining which player goes first but before drawing any cards, each player places one random card from their deck into, when playing for ante. The winner of the game becomes owner of any cards in the ante zone."@en ;
  skos:prefLabel "Ante Zone"@en ;
  skos:note "The ante zone does not get used much, is considered an optional rule, and probably only still exists in the rules because certain cards from early on in the game's history make reference to it" ;
  skos:note "CR 407" ;
.

:0000022 
  a owl:Class ;
  rdfs:subClassOf ??? ;
  rdfs:label "MTG Mana"@en ;
  skos:definition "Mana is a..."@en ;
  skos:prefLabel "Mana"@en ;
  skos:note "Mana is a problem. It is a resource generated by objects' mana abilities, stored in a players' mana pool, and can be used to cast spells and activate abilities, but it never gets represented by anything on the tabletop, or outside of players' minds. It should maybe be defined as a measurement of some kind." ;
.

:0000023 
  a owl:Class ;
  rdfs:subClassOf cco:InformationContentEntity ; 
  rdfs:label "MTG Object Characteristic" ;
  skos:definition "A characteristic is any one of the following Information Content Entities that can be borne by an MTG object: name, mana cost, color, color indicator, card type, subtype, supertype, rules text, abilities, power, toughness, loyalty, defense, hand modifier, and life modifier."@en ;
  skos:altLabel "Object Characteristic"@en ;
  skos:prefLabel "Characteristic"@en ;
  skos:note "CR 109.3" ;
  skos:note "I can see problems with this and with copies, at least, because while characteristics do seem obviously to be information entities (as the Comprehensive Rules insist) it is difficult to see how some characteristics have a generic dependence relation to the appropriate object when some objects are only imagined by players." ;
. 

:0000024
  a owl:Class ;
  rdfs:subClassOf :0000023 ;
  rdfs:label "MTG name"@en ;
  skos:definition "A name is an object characteristic whose information content is some word or phrase which refers to the object either in virtue of being printed in the top left corner of the card or determined by some ability or effect which brings the object into existence or changes its name."@en ;
  skos:prefLabel "Name"@en ;
  skos:note "A clumsy definition, but remember: cards have names printed on them, some cards can become copies or clones of other cards, and tokens are all created with a name (which is the same as their creature types in most cases)." ; 
.

:0000025
a owl:Class ;
rdfs:subClassOf :0000023 ;
rdfs:label "MTG Mana Cost"@en ;
skos:definition "A mana cost is an object characteristic whose information content is the amount and color of mana required to play the object from a player's hand."@en ;
skos:prefLabel "Mana Cost"@en ;
skos:note "mana cost also determines the color(s) of a card, as well as whether it is mono- or multicolored." ;
skos:note "there is a question of whether it should be described as playing an object/card or casting a spell/object/card." ;
.

:0000026 
  a owl:Class ;
  rdfs:subClassOf :0000023 ;
  rdfs:label "MTG Color"@en ;
  skos:definition "A color is an object characteristic determined by the object's mana cost or color indicator, whose information content is at least one of either White, Green, Red, Black, Blue, or Colorless."@en ;
  skos:prefLabel "Color"@en ;
  skos:note "Need to check on the status of Colorless as an object's color. This may be a tricky issue." ;
  skos:note "Not sure whether to include a corresponding quality class." ;
.

:0000027 
  a owl:Class ;
rdfs:subClassOf :0000023 ;
rdfs:label "MTG Color Indicator"@en ;
skos:definition "A Color Indicator is an object characteristic whose information content is the color(s) of the object."@en ;
skos:prefLabel "Color Indicator"@en ;
.

:0000028 
  a owl:Class ;
  rdfs:subClassOf :0000023 ;
  rdfs:label "MTG Card Type"@en ;
  skos:definition "A card type is an object characteristic whwhich is part of a card's type line and which determines several aspects of how that card can interact with the rules of the game."@en ;
  skos:prefLabel "Card Type"@en ;
.

:0000029 
  a owl:Class ;
  rdfs:subClassOf :0000023 ;
  rdfs:label "MTG Card Subtype"@en ;
  skos:definition "A card subtype is an object characteristic whose information content is..."@en ;
  skos:prefLabel "Card Subtype"@en ;
.

:0000030 
  a owl:Class ;
  rdfs:subClassOf :0000023 ;
  rdfs:label "MTG Card Supertype"@en ;
  skos:prefLabel "Card Supertype"@en ;
  skos:definition "A card supertype is an object characteristic whose information content is..."@en ;
.

:0000031 
   a owl:Class ;
  owl:disjointWith :0000045 ;
  rdfs:subClassOf :0000023 ,
    [rdf:type owl:Restriction ;
              owl:onProperty obo:BFO_0000176 ;
              owl:SomeValuesFrom :0000044
    ] ;
  rdfs:label "MTG Object Rules Text"@en ;
  skos:definition "Rules text is an object characteristic which is part of an object's text box and which has game-mechanical effect(s)."@en ;
  skos:prefLabel "Rules Text"@en ;
.

:0000032 
  a owl:Class ;
  rdfs:subClassOf :0000023 ;
  rdfs:label "MTG Object Ability Information"@en ;
  skos:definition "Object ability information is an object characteristic which is some portion of its rules text, delineated from other portions by a paragraph break."@en ;
  skos:prefLabel "Ability"@en ;
  skos:note "Not sure whether this should strictly be a subclass of :0000023 or whether it should simply be a part of a text box." ;
.

:0000033 
  a owl:Class ;
  rdfs:subClassOf :0000023 ;
  rdfs:label "MTG Power"@en ;
  skos:definition "Power is an object characteristic which determines how much damage a creature deals in combat."@en ;
  skos:prefLabel "Power"@en ;
.

:0000034 
  a owl:Class ;
  rdfs:subClassOf :0000023 ;
  rdfs:label "MTG Toughness"@en ;
  skos:definition "Toughness is an object characteristic which determines how much damage a creature can sustain before it is destroyed."@en ;
  skos:prefLabel "Toughness"@en ;
.

:0000035 
  a owl:Class ;
  rdfs:subClassOf :0000023 ;
  rdfs:label "MTG Loyalty"@en ;
  skos:definition "Loyalty is an object characteristic which determines how many loyalty counters a planeswalker comes into play with."@en ;
  skos:prefLabel "Loyalty"@en ;
.

:0000036
  a owl:Class ;
  rdfs:subClassOf :0000023 ;
  rdfs:label "MTG Hand Modifier"@en ;
  skos:definition "A hand modifier is an object characteristic of a Vanguard card which alters its owner's starting hand size and maximum hand size at the start of a Vanguard game."@en ;
  skos:prefLabel "Hand Modifier"@en ;
  skos:note "CR 313.6" ;
.

:0000037 
  a owl:Class ;
  rdfs:subClassOf :0000023 ;
  rdfs:label "MTG Life Modifier"@en ;
  skos:definition "A life modifier is an object characteristic of a Vanguard card whch alters its owner's life total at the start of a Vanguard game."@en ;
  skos:prefLabel "Life Modifier"@en ;
  skos:note "CR 313.7" ;
. 

:0000038 
  a owl:Class ;
  rdfs:subClassOf :0000029
  rdfs:label "MTG Creature Subtype"@en ;
  skos:definition "A creature type is an object characteristic which is a part of an object's type line and which determines whether and how that object can be targeted or affected by spells and abilities."@en ;
  skos:prefLabel "Creature Type"@en ;
.

:0000039
  a owl:Class ;
  rdfs:subClassOf :0000029 
  rdfs:label "MTG Land Subtype"@en ;
  skos:definition "A Land type is an object characteristic which is part of an object's type line and which determines what color of mana that land can produce in addition to whether and how that object can be targeted or affected by spells and abilities."@en ;
  skos:prefLabel "Land Type"@en ;
. 

:0000040 
  a owl:Class ;
  rdfs:subClassOf :0000029 ;
  rdfs:label "MTG Enchantment Subtype"@en ;
  skos:prefLabel "Enchantment Type"@en ;
  skos:definition "An enchantment type is an object characteristic which is part of an object's type line and which determines various game-mechanical functions of the object in addition to whether and how that object can be targeted or affected by spells and abilities."@en ;
.

:0000041
  a owl:Class ;
  rdfs:subClassOf :0000029 ;
  rdfs:label "MTG Artifact Subtype"@en ;
  skos:prefLabel "Artifact Type"@en ;
.

:0000042 
  a owl:Class ;
  rdfs:subClassOf :0000029 ;
  rdfs:label "MTG Planeswalker Subtype"@en ;
  skos:prefLabel "Planeswalker Type"@en ;
.

:0000043 
  a owl:Class ;
  rdfs:subClassOf :0000029 ;
  rdfs:label "MTG Spell Subtype"@en ;
  skos:prefLabel "Spell Type"@en ;
.

:0000044
  a owl:Class ;
  rdfs:subClassOf cco:InformationContentEntity ;
  rdfs:label "MTG Text Box"@en ;
  skos:definition "A text box is an information content entity whose content is the sum of any rules text or flavor text on an object."@en ;
  skos:prefLabel "Text Box"@en ;
.

:0000045 
  a owl:Class ;
  owl:disjointWith 0000031 ;
  rdfs:subClassOf cco:InformationContentEntity ,
          [rdf:type owl:Restriction ;
              owl:onProperty obo:BFO_0000176 ;
              owl:SomeValuesFrom :0000044
    ] ;
  rdfs:label "MTG Flavor Text"@en ;
  skos:definition "Flavor text is an information content entity whose content is italicized text which serves merely to add artistic appeal to the game."@en ;
  skos:prefLabel "Flavor Text"@en ;
  skos:note "CR 207.2b" ;
.

:0000046 
  a owl:Class ;
  rdfs:subClassOf cco:InformationContentEntity ,
          [rdf:type owl:Restriction ;
              owl:onProperty obo:BFO_0000176 ;
              owl:someValuesFrom :0000044
    ] ;
  rdfs:label "MTG Reminder Text"@en ;
  skos:definition "Reminder text is an information content entity whose content is italicized text which serves as a reminder for what certain keywords and other technical Magic-related terms mean."@en ;
  skos:note "CR 207.2" ;
.
##################
#Object Properties
##################

